DescriptionToFunction.v
@@ -1,0 +1,30 @@
+Require Export Parser.NetworkProperties.
+Require Export Parser.Cast.
+
+Open Scope nat_scope.
+
+Opaque range.
+
+(** `build_fun` constructs a progatator network from a description `descr`, and
+    after running it, extract the value for the cell corresponding to the syntax
+    s *)
+Program Definition build_fun { G } (descr: Description G) { A } (s: Syntax A): option (G A) :=
+  let num_cells: nat := sum_sizes vars + syntax_size s in
+  let N' := compute_cells num_cells (make_network s descr) (range 0 num_cells) _ in
+  let s: node_type A G := cast _ (state (cells N' (sum_sizes vars))) in
+  snd s.
+
+Next Obligation.
+  repeat light || destruct_proj1_sigs || rewrite range_spec in *;
+    eauto using io_types_make_network;
+    eauto using max_pointer_make_network.
+Qed.
+
+Next Obligation.
+  rewrite cell_type_compute_cells.
+  unfold make_network.
+  rewrite cell_make_network';
+    eauto using cell_type_node_type.
+Qed.
+
+Fail Next Obligation. (* no more obligations for build_fun *)
