NetworkWipCells.v
@@ -1,0 +1,474 @@
+Require Import Coq.Strings.String.
+Require Import Coq.Lists.List.
+Import ListNotations.
+
+Require Import PeanoNat.
+
+Require Export Parser.DescriptionInd.
+Require Export Parser.NetworkGoodCells.
+Require Export Parser.NetworkProperties.
+
+Opaque Nat.eq_dec.
+
+Definition wip_inputs
+             { A } (s: Syntax A) { G } (descr: Description G) (N: Network) k (b1 b2: nat): Prop :=
+  match s with
+  | Epsilon _ => inputs N k = []
+  | Failure _ => inputs N k = []
+  | Elem _ => inputs N k = []
+  | Disjunction s1 s2 => exists opt1 opt2,
+      b1 < S k /\
+      S (k + syntax_size s1) < b2 /\
+      inputs N k = [ S k; S (k + syntax_size s1) ] /\
+      map (cells N) (inputs N k) = [
+        make_cell_with_state s1 descr opt1; make_cell_with_state s2 descr opt2
+      ]
+  | Sequence s1 s2 => exists opt1 opt2,
+      b1 <= S k /\
+      S (k + syntax_size s1) < b2 /\
+      inputs N k = [ S k; S (k + syntax_size s1) ] /\
+      map (cells N) (inputs N k) = [
+        make_cell_with_state s1 descr opt1; make_cell_with_state s2 descr opt2
+      ]
+  | Map f g s' => exists opt',
+      b1 <= S k /\ S k < b2 /\
+      inputs N k = [ S k ] /\
+      map (cells N) (inputs N k) = [ make_cell_with_state s' descr opt' ]
+  | Var x => exists opt',
+      inputs N k = [ sum_sizes_until x ] /\
+      map (cells N) (inputs N k) = [ make_cell_with_state (e x) descr opt' ]
+  end.
+
+Definition wip_cell { G } (descr: Description G) (N: Network) (k: nat) (b1 b2: nat): Prop :=
+  exists A (s: Syntax A) (opt: option (G A)),
+    cells N k = make_cell_with_state s descr opt /\
+    opt_forall opt (descr_ind descr s) /\
+    wip_inputs s descr N k b1 b2.
+
+(** The "work-in-progress" property states that the state of every cell can
+    be derived from the states of its inputs according to the description `descr`.
+    We prove later that this is an invariant of the network (during computation),
+    which ensures the soundness statement `fun_soundness_statement` *)
+Definition wip_cells { G } (descr: Description G) (N: Network) (b1 b2: nat): Prop :=
+  forall k, b1 <= k -> k < b2 -> wip_cell descr N k b1 b2.
+
+Ltac instantiate_wip_cells k :=
+  match goal with
+  | H: wip_cells _ _ _ _ |- _ =>
+    poseNew (Mark k "instantiate_wip_cells");
+    let W := fresh "W" in
+    unshelve epose proof (H k _ _) as W; eauto with lia; unfold wip_cell in W
+  end.
+
+Lemma good_inputs_wip_inputs:
+  forall A (s: Syntax A) G (descr: Description G) N k b1 b2,
+    good_inputs s descr N k b1 b2 ->
+    (forall x, cells N (sum_sizes_until x) = make_cell_with_state (e x) descr None) ->
+    wip_inputs s descr N k b1 b2.
+Proof.
+  destruct s; repeat light; eauto 6.
+  exists None; repeat light || rewrite_known_inputs.
+Qed.
+
+Lemma good_cell_wip_cell:
+  forall G (descr: Description G) N k b1 b2,
+    good_cell descr N k b1 b2 ->
+    (forall x, cells N (sum_sizes_until x) = make_cell_with_state (e x) descr None) ->
+    wip_cell descr N k b1 b2.
+Proof.
+  unfold good_cell, wip_cell;
+    repeat light.
+  exists A, s, None; repeat light;
+    eauto using good_inputs_wip_inputs.
+Qed.
+
+(** Initially, the network satisfies the `wip_cells` invariant *)
+Lemma wip_cells_make_network:
+  forall A (s: Syntax A) G (descr: Description G) k,
+    k < sum_sizes vars + syntax_size s ->
+    wip_cell descr (make_network s descr) k 0 (sum_sizes vars + syntax_size s).
+Proof.
+  intros; apply good_cell_wip_cell;
+    eauto using good_cells_make_network;
+    eauto using var_cells_make_network.
+Qed.
+
+
+Lemma still_wip_inputs:
+  forall A (s: Syntax A) G (descr: Description G) N b1 b2 k opt (opt': option (G A)) H,
+    wip_inputs s descr N k b1 b2 ->
+    cells N k = make_cell_with_state s descr opt ->
+    (forall x, exists optx, cells N (sum_sizes_until x) = make_cell_with_state (e x) descr optx) ->
+    wip_inputs s descr (
+      set_cell N k {|
+       main_type := main_type (cells N k);
+       cell_type := cell_type (cells N k);
+       input_types := input_types (cells N k);
+       update := update (cells N k);
+       measure := measure (cells N k);
+       state := cast H (s, opt')
+      |})
+      k b1 b2.
+Proof.
+  destruct s; repeat light.
+  - eexists; eexists; repeat light || map_ext_in || destruct_match || rewrite_known_inputs;
+      eauto; try lia.
+  - eexists; eexists; repeat light || map_ext_in || destruct_match || rewrite_known_inputs;
+      eauto; try lia.
+  - eexists; repeat light || map_ext_in || destruct_match || rewrite_known_inputs;
+      eauto; try lia.
+  - pose proof (Nat.eq_dec k (sum_sizes_until x)); lights;
+      try solve [ eexists; repeat light || destruct_match || rewrite_known_inputs; eauto ].
+    specialize H2 with x; lights.
+    pose proof (eq_trans (eq_sym H1) H0) as HE.
+    pose proof (f_equal_dep _ state HE);
+      repeat eq_dep || cbn in * || rewrite state_make_cell in * || invert_constructor_equalities.
+    exists opt'; repeat light || rewrite_known_inputs || destruct_match || invert_constructor_equalities.
+    f_equal.
+    generalize H.
+    rewrite H3; repeat cbn in * || eq_dep.
+    repeat rewrite <- H6 || light || eq_dep.
+Qed.
+
+Lemma still_wip_inputs2:
+  forall A (s: Syntax A) G (descr: Description G) N b1 b2 k k' hl,
+    wip_inputs s descr N k b1 b2 ->
+    k <> k' ->
+    wip_inputs s descr (
+      set_cell N k' {|
+       main_type := main_type (cells N k');
+       cell_type := cell_type (cells N k');
+       input_types := input_types (cells N k');
+       update := update (cells N k');
+       measure := measure (cells N k');
+       state := update (cells N k') hl
+      |})
+      k b1 b2.
+Proof.
+  destruct s; repeat light || rewrite_known_inputs || invert_constructor_equalities.
+  - destruct (Nat.eq_dec k' (S k)); destruct (Nat.eq_dec k' (S (k + syntax_size s1)));
+      repeat light;
+      try solve [ repeat syntax_size_gt_0; eauto with lia ].
+
+    + unshelve eexists (@snd (Syntax A) (option (G A)) (cast _ (update (cells N (S k)) hl)));
+        try solve [ rewrite_any; eapply cell_type_node_type ].
+      exists opt2; repeat light || f_equal;
+        eauto using update_make_cell2.
+
+    + exists opt1;
+      unshelve eexists (@snd (Syntax A) (option (G A)) (cast _ (update (cells N (S (k + syntax_size s1))) hl)));
+        try solve [ rewrite_any; eapply cell_type_node_type ];
+        repeat light || f_equal;
+        eauto using update_make_cell2.
+
+    + exists opt1, opt2; repeat light || f_equal.
+
+  - destruct (Nat.eq_dec k' (S k)); destruct (Nat.eq_dec k' (S (k + syntax_size s1)));
+      repeat light;
+      try solve [ repeat syntax_size_gt_0; eauto with lia ].
+
+    + unshelve eexists (@snd (Syntax A) (option (G A)) (cast _ (update (cells N (S k)) hl)));
+        try solve [ rewrite_any; eapply cell_type_node_type ].
+      exists opt2; repeat light || f_equal;
+        eauto using update_make_cell2.
+
+    + exists opt1;
+      unshelve eexists (@snd (Syntax B) (option (G B)) (cast _ (update (cells N (S (k + syntax_size s1))) hl)));
+        try solve [ rewrite_any; eapply cell_type_node_type ];
+        repeat light || f_equal;
+        eauto using update_make_cell2.
+
+    + exists opt1, opt2; repeat light || f_equal.
+
+  - destruct (Nat.eq_dec k' (S k));
+      repeat light.
+
+    + unshelve eexists (@snd (Syntax A) (option (G A)) (cast _ (update (cells N (S k)) hl)));
+        try solve [ rewrite_any; eapply cell_type_node_type ];
+        repeat light || f_equal;
+        eauto using update_make_cell2.
+
+    + exists opt';
+        repeat light || f_equal;
+        eauto using update_make_cell2.
+
+  - destruct (Nat.eq_dec k' (sum_sizes_until x));
+      repeat light.
+
+    + unshelve eexists (@snd (Syntax (get_type x)) (option (G (get_type x))) (cast _ (update (cells N (sum_sizes_until x)) hl)));
+        try solve [ rewrite_any; eapply cell_type_node_type ];
+        repeat light || f_equal;
+        eauto using update_make_cell2.
+
+    + exists opt';
+        repeat light || f_equal;
+        eauto using update_make_cell2.
+Qed.
+
+Ltac equate_states :=
+  match goal with
+  | H1: state (cells ?N ?k) = ?q1,
+    H2: state (cells ?N ?k) = ?q2 |- _ =>
+    poseNew (Mark (H1, H2) "equate_states");
+    pose proof (eq_trans (eq_sym H1) H2)
+  end.
+
+Lemma update_obligation:
+  forall A (s: Syntax A) G (descr : Description G) (N : Network) (k : nat) (opt: option (G A)),
+    cells N k = make_cell_with_state s descr opt ->
+    (Syntax A * option (G A))%type = cell_type (cells N k).
+Proof.
+  repeat light || f_equal_dep.
+  rewrite_known_cells.
+  rewrite cell_type_node_type.
+  reflexivity.
+Qed.
+
+Lemma update_is_cast:
+  forall A (s: Syntax A) G (descr : Description G) (N : Network) (k : nat) (opt: option (G A)) hl
+    (H: cells N k = make_cell_with_state s descr opt),
+    exists opt': option (G A),
+      update (cells N k) hl = cast (update_obligation A s G descr N k opt H) (s, opt').
+Proof.
+  repeat light || f_equal_dep.
+  destruct s;
+    repeat light || rewrite_known_updates || eq_dep;
+    try solve [
+      repeat generalize_proofs; generalize hl;
+      rewrite_known_cell_types;
+      rewrite H5; repeat light || eq_dep;
+      unfold rules_to_update; eauto
+    ].
+Qed.
+
+(** The "work-in-progress" invariant is maintained after running the network one step *)
+Lemma wip_cells_compute_cell:
+  forall G (descr: Description G) N N' b1 b2 k pre,
+    wip_cells descr N b1 b2 ->
+    b1 <= k ->
+    k < b2 ->
+    (forall x, b1 <= sum_sizes_until x /\ sum_sizes_until x < b2) ->
+    (forall x, exists optx, cells N (sum_sizes_until x) = make_cell_with_state (e x) descr optx) ->
+    compute_cell N k pre = Some N' ->
+    wip_cells descr N' b1 b2.
+Proof.
+  unfold compute_cell, wip_cells, wip_cell;
+    repeat light || destruct_match || invert_constructor_equalities || clear l matched ||
+           instantiate_any ||
+           lazymatch goal with
+           | H: cells ?N ?k = make_cell_with_state ?s _ _ |- exists _ _ _, {| cell_type := cell_type (cells ?N ?k); state := ?q |} = _ /\ _ =>
+             eexists _; exists s; unshelve eexists (snd (@cast _ (node_type _ G) _ q))
+           end;
+      try solve [ rewrite_known_cells; eauto using cell_type_node_type ];
+      eauto using update_make_cell;
+      eauto using still_wip_inputs;
+      try solve [ repeat eexists; eauto using still_wip_inputs2 ].
+
+  - repeat f_equal_dep.
+    repeat eq_dep.
+
+    unfold make_cell_with_state in H13, H15, H17.
+    destruct s0; rewrite H15; repeat light || eq_dep;
+    try solve [
+      repeat generalize_proofs;
+      rewrite_known_inputs; cbn;
+      match goal with
+      | H: input_types (cells _ _) = _ |- _ => rewrite H
+      end; cbn;
+      match goal with
+      | H: cell_type (cells _ _) = _ |- _ => rewrite H
+      end; cbn;
+      unfold opt_forall; repeat light || eq_dep || destruct_match;
+      apply_anywhere fold_left_or_else; repeat light; eauto with descr_ind
+    ].
+
+    + (* disjunction *)
+      repeat generalize_proofs.
+      rewrite_known_inputs; repeat cbn in * || invert_constructor_equalities.
+      unshelve epose proof (H (S k0) _ _); try lia; repeat destruct_exists || destruct_and.
+      unshelve epose proof (H (S (k0 + syntax_size s0_1)) _ _); try lia;
+        repeat destruct_exists || destruct_and.
+      match goal with
+      | H: input_types (cells _ _) = _ |- _ => rewrite H
+      end; cbn.
+
+      repeat rewrite_known_cell_types.
+      repeat f_equal_dep2.
+      rewrite cell_type_node_type in *.
+      rewrite state_make_cell in *.
+      repeat cbn in * || eq_dep.
+      repeat rewrite_known_states; repeat cbn in * || eq_dep.
+      repeat generalize_proofs.
+
+      repeat rewrite_known_cell_types; repeat light || eq_dep.
+      unfold opt_forall; repeat light || eq_dep || destruct_match.
+      apply_anywhere fold_left_or_else; repeat light.
+      eapply in_disj_descr; eauto;
+        unfold node_type; repeat light || eq_dep.
+      * repeat same_cell_same_type; repeat light || eq_dep.
+        repeat equate_states.
+        repeat equate_states; repeat apply_anywhere eq_rect_reverse;
+          repeat light || invert_constructor_equalities.
+      * repeat same_cell_same_type; repeat light || eq_dep.
+        repeat equate_states; repeat apply_anywhere eq_rect_reverse;
+          repeat light || invert_constructor_equalities.
+
+    + (* sequence *)
+      repeat generalize_proofs.
+      rewrite_known_inputs; repeat cbn in * || invert_constructor_equalities.
+      unshelve epose proof (H (S k0) _ _); try lia; repeat destruct_exists || destruct_and.
+      unshelve epose proof (H (S (k0 + syntax_size s0_1)) _ _); try lia;
+        repeat destruct_exists || destruct_and.
+      match goal with
+      | H: input_types (cells _ _) = _ |- _ => rewrite H
+      end; cbn.
+
+      repeat rewrite_known_cell_types.
+      repeat f_equal_dep2.
+      rewrite cell_type_node_type in *.
+      rewrite state_make_cell in *.
+      repeat cbn in * || eq_dep.
+      repeat rewrite_known_states; repeat cbn in * || eq_dep.
+      repeat generalize_proofs.
+
+      repeat rewrite_known_cell_types; repeat light || eq_dep.
+      unfold opt_forall; repeat light || eq_dep || destruct_match.
+      apply_anywhere fold_left_or_else; repeat light.
+      eapply in_seq_descr; eauto;
+        unfold node_type; repeat light || eq_dep.
+      * repeat same_cell_same_type; repeat light || eq_dep.
+        repeat equate_states; repeat apply_anywhere eq_rect_reverse;
+          repeat light || invert_constructor_equalities.
+      * repeat same_cell_same_type; repeat light || eq_dep.
+        repeat equate_states; repeat apply_anywhere eq_rect_reverse;
+          repeat light || invert_constructor_equalities.
+
+    + (* map *)
+      repeat generalize_proofs.
+      rewrite_known_inputs; repeat cbn in * || invert_constructor_equalities.
+      unshelve epose proof (H (S k0) _ _); try lia; repeat destruct_exists || destruct_and.
+      match goal with
+      | H: input_types (cells _ _) = _ |- _ => rewrite H
+      end; cbn.
+
+      repeat rewrite_known_cell_types.
+      repeat f_equal_dep2.
+      rewrite cell_type_node_type in *.
+      rewrite state_make_cell in *.
+      repeat cbn in * || eq_dep.
+      repeat rewrite_known_states; repeat cbn in * || eq_dep.
+      repeat generalize_proofs.
+
+      repeat rewrite_known_cell_types; repeat light || eq_dep.
+      unfold opt_forall; repeat light || eq_dep || destruct_match.
+      apply_anywhere fold_left_or_else; repeat light.
+      eapply in_map_descr; eauto;
+        unfold node_type; repeat light || eq_dep.
+      repeat same_cell_same_type; repeat light || eq_dep.
+      repeat equate_states; repeat apply_anywhere eq_rect_reverse;
+        repeat light || invert_constructor_equalities.
+
+    + (* var *)
+      repeat generalize_proofs.
+      rewrite_known_inputs; repeat cbn in * || invert_constructor_equalities.
+      unshelve epose proof (H (sum_sizes_until x) _ _);
+        try lia; repeat destruct_exists || destruct_and || apply_any.
+      match goal with
+      | H: input_types (cells _ _) = _ |- _ => rewrite H
+      end; cbn.
+
+      repeat rewrite_known_cell_types.
+      repeat f_equal_dep2.
+      rewrite cell_type_node_type in *.
+      rewrite state_make_cell in *.
+      repeat cbn in * || eq_dep.
+      repeat rewrite_known_states; repeat cbn in * || eq_dep.
+      repeat generalize_proofs.
+
+      repeat rewrite_known_cell_types; repeat light || eq_dep.
+      unfold opt_forall; repeat light || eq_dep || destruct_match.
+      apply_anywhere fold_left_or_else; repeat light.
+      eapply in_var_descr; eauto;
+        unfold node_type; repeat light || eq_dep.
+      repeat same_cell_same_type; repeat light || eq_dep.
+      repeat equate_states; repeat apply_anywhere eq_rect_reverse;
+        repeat light || invert_constructor_equalities.
+
+  - match goal with
+    | |- context[update ?c ?hl] =>
+      unshelve epose proof (update_is_cast _ _ _ _ _ _ _ hl H10)
+    end; lights.
+    rewrite H11; eauto using still_wip_inputs.
+Qed.
+
+Opaque make_cell_with_state.
+Opaque compute_cells.
+
+Lemma wip_cells_compute_cells':
+  forall m G (descr: Description G) N num_cells ks pre,
+    (sum_measures num_cells N, length ks) = m ->
+    wip_cells descr N 0 num_cells ->
+    (forall k, In k ks -> k < num_cells) ->
+    (forall x, sum_sizes_until x < num_cells) ->
+    (forall x, exists optx, cells N (sum_sizes_until x) = make_cell_with_state (e x) descr optx) ->
+    wip_cells descr (compute_cells num_cells N ks pre) 0 num_cells.
+Proof.
+  induction m using measure_induction; destruct ks;
+    repeat light || compute_cells_def || destruct_match || options.
+
+  - clear matched.
+    revert i.
+    generalize (PropagatorNetwork.compute_cells_obligations_obligation_3 num_cells N n ks pre).
+    generalize (PropagatorNetwork.compute_cells_obligations_obligation_2 num_cells N n ks pre).
+    generalize (PropagatorNetwork.compute_cells_obligations_obligation_1 num_cells N n ks pre).
+    repeat light || destruct_match || options.
+
+    eapply H;
+      repeat light;
+      try solve [ apply left_lex; eauto using compute_cell_size ].
+
+    + eapply (wip_cells_compute_cell _ _ N _ _ _ n);
+        eauto; repeat light || apply_any; try lia.
+    + specialize H4 with x; lights; eauto using compute_cell_still_make_cell.
+
+  - clear matched.
+    revert n0.
+    generalize (PropagatorNetwork.compute_cells_obligations_obligation_5 num_cells N n ks pre).
+    generalize (PropagatorNetwork.compute_cells_obligations_obligation_1 num_cells N n ks pre).
+    repeat light || destruct_match;
+      eauto 2 with lights.
+
+    eapply H;
+      repeat light || apply right_lex;
+      eauto using cell_type_compute_cell.
+Qed.
+
+(** The "work-in-progress" invariant is maintained after running the network *)
+Lemma wip_cells_compute_cells:
+  forall G (descr: Description G) N num_cells ks pre,
+    wip_cells descr N 0 num_cells ->
+    (forall k, In k ks -> k < num_cells) ->
+    (forall x, sum_sizes_until x < num_cells) ->
+    (forall x, exists optx, cells N (sum_sizes_until x) = make_cell_with_state (e x) descr optx) ->
+    wip_cells descr (compute_cells num_cells N ks pre) 0 num_cells.
+Proof.
+  eauto using wip_cells_compute_cells'.
+Qed.
+
+Lemma wip_cells_compute_cells_make_network:
+  forall A (s: Syntax A) G (descr: Description G) pre,
+    wip_cells descr (
+      compute_cells
+        (sum_sizes vars + syntax_size s)
+        (make_network s descr)
+        (range 0 (sum_sizes vars + syntax_size s))
+        pre
+    ) 0 (sum_sizes vars + syntax_size s).
+Proof.
+  intros.
+  apply wip_cells_compute_cells;
+    repeat light || unfold wip_cells;
+    try solve [ pose proof (sum_sizes_until_sum_sizes x); eauto with lia ];
+    eauto using wip_cells_make_network;
+    eauto using var_cells_make_network.
+Qed.
